src/Core/Solver/Context/DG/Call_String_Collecting_Refinement.thy
@@ -67,17 +67,17 @@ text \<open>
 
 lemma call_string_collecting_mono:
   assumes le: "k1 \<le> k2"
-  shows "activation_collect gs (cs_enterc k2) seed g S v c2
-           \<subseteq> activation_collect gs (cs_enterc k1) (take k1 seed) g S v (take k1 c2)"
+  shows "activation_collect gs (cs_enterc k2) seed (=) g S v c2
+           \<subseteq> activation_collect gs (cs_enterc k1) (take k1 seed) (=) g S v (take k1 c2)"
 proof
-  fix s assume "s \<in> activation_collect gs (cs_enterc k2) seed g S v c2"
+  fix s assume "s \<in> activation_collect gs (cs_enterc k2) seed (=) g S v c2"
   then obtain t where t1: "t \<in> valid_ltr gs g S" and t2: "sink_node t = v"
     and t3: "key (cs_enterc k2) seed t = c2" and t4: "sink_store t = s"
     by (rule activation_collect_E)
   from key_cs_enterc_k_mono[OF le, of seed t] t3
   have key1: "key (cs_enterc k1) (take k1 seed) t = take k1 c2" by simp
-  show "s \<in> activation_collect gs (cs_enterc k1) (take k1 seed) g S v (take k1 c2)"
-    using activation_collect_I[OF t1 t2 key1] t4 by simp
+  show "s \<in> activation_collect gs (cs_enterc k1) (take k1 seed) (=) g S v (take k1 c2)"
+    using activation_collect_I[where ctx_rep = "(=)", OF t1 t2 key1] t4 by simp
 qed
 
 end
